Updating manifest generator to use the CompMap structure

src/Manifest.v
@@ -56,13 +56,14 @@ Global Instance jsonifiable_ASP_Locator : Jsonifiable ASP_Locator :=
 
 Definition PolicyT := list (Plc * ASP_ID).
 
+Definition ASP_Compat_MapT := MapC ASP_ID ASP_ID.
 
 (** [Manifest] defines an attestation manger, a list of ASPs, and other
    * managers it is aware of (a single AM and its interconnections).
    *)
   Record Manifest := {
     asps              : manifest_set ASP_ID; 
-    ASP_Compat_Map    : MapC ASP_ID ASP_ID;
+    ASP_Compat_Map    : ASP_Compat_MapT;
     ASP_Mapping       : MapC ASP_ID FS_Location;
     man_policy        : PolicyT  ;
     (* TO DO: Add privacy and selection policies to manifest? *)
