src/Manifest_Generator.v
@@ -15,100 +15,24 @@ Require Import List.
 Import ListNotations.
 
 Definition aspid_manifest_update (i:ASP_ID) (m:Manifest) : Manifest := 
-  let '{| my_abstract_plc := oldPlc;
-          asps := oldasps; 
-          uuidPlcs := oldKnowsOf; 
-          pubKeyPlcs := oldContext; 
-          targetPlcs := oldTargets ;
-          policy := oldPolicy |} := m in
-  (Build_Manifest oldPlc (manset_add i oldasps) oldKnowsOf oldContext oldTargets oldPolicy).
-
-Definition knowsof_manifest_update (toPlc:Plc) (m:Manifest) : Manifest := 
-    let '{| my_abstract_plc := oldPlc;
-            asps := oldasps; 
-            uuidPlcs := oldKnowsOf; 
-            pubKeyPlcs := oldContext; 
-            targetPlcs := oldTargets ;
-            policy := oldPolicy |} := m in
-    (Build_Manifest oldPlc oldasps (manset_add toPlc oldKnowsOf) oldContext oldTargets oldPolicy).
-
-Definition knowsof_myPlc_manifest_update (m:Manifest) : Manifest :=
-  knowsof_manifest_update (my_abstract_plc m) m.
-
-Definition myPlc_manifest_update (p:Plc) (m:Manifest) : Manifest := 
-  let '{| my_abstract_plc := _;
-          asps := oldasps; 
-          uuidPlcs := oldKnowsOf; 
-          pubKeyPlcs := oldContext; 
-          targetPlcs := oldTargets; 
-          policy := oldPolicy |} := m in
-  (Build_Manifest p oldasps oldKnowsOf oldContext oldTargets oldPolicy).
-
-Definition pubkey_manifest_update (p:Plc) (m:Manifest) : Manifest := 
-  let '{| my_abstract_plc := oldPlc;
-          asps := oldasps; 
-          uuidPlcs := oldKnowsOf; 
-          pubKeyPlcs := oldContext; 
-          targetPlcs := oldTargets ;
-          policy := oldPolicy |} := m in
-  (Build_Manifest oldPlc oldasps oldKnowsOf (manset_add p oldContext) oldTargets oldPolicy).
-
-Definition pubkeys_manifest_update_replace_all (ps:manifest_set Plc) (m:Manifest) : Manifest := 
-        let '{| my_abstract_plc := oldMyPlc;
-                asps := oldasps; 
-                uuidPlcs := oldKnowsOf; 
-                pubKeyPlcs := _; 
-                targetPlcs := oldTargets ;
-                policy := oldPolicy |} := m in
-        (Build_Manifest oldMyPlc oldasps oldKnowsOf ps oldTargets oldPolicy).
-
-Definition pubkeys_manifest_update (ps:manifest_set Plc) (m:Manifest) : Manifest := 
-  let '{| my_abstract_plc := oldMyPlc;
-          asps := oldasps; 
-          uuidPlcs := oldKnowsOf; 
-          pubKeyPlcs := oldPubs; 
-          targetPlcs := oldTargets ;
-          policy := oldPolicy |} := m in
-  (Build_Manifest oldMyPlc oldasps oldKnowsOf (fold_right manset_add oldPubs ps) oldTargets oldPolicy).
-
-Definition update_manifest_policy_targ (targp:Plc) (targid:Plc) (m:Manifest) : Manifest :=
-  let '{| my_abstract_plc := oldMyPlc;
-          asps := oldasps; 
-          uuidPlcs := oldKnowsOf; 
-          pubKeyPlcs := oldContext ; 
-          targetPlcs := oldTargets ;
-          policy := oldPolicy |} := m in
-  (Build_Manifest oldMyPlc oldasps oldKnowsOf oldContext (manset_add targp oldTargets) oldPolicy).
-
+  let '{| asps := oldasps; 
+          ASP_Compat_Map := oldCompatMap;
+          ASP_Mapping := oldFSMap;
+          man_policy := oldPolicy |} := m in
+  (Build_Manifest (manset_add i oldasps) oldCompatMap oldFSMap oldPolicy).
   
 Definition asp_manifest_update (a:ASP) (m:Manifest) : Manifest :=
   match a with 
   | ASPC _ _ params => 
       match params with
-      | asp_paramsC i _ targp targid => 
-        let m' := update_manifest_policy_targ targp targid m in
-          aspid_manifest_update i m'
+      | asp_paramsC i _ _ _ => aspid_manifest_update i m
       end
   | SIG => aspid_manifest_update (sig_aspid) m
   | HSH => aspid_manifest_update (hsh_aspid) m
-  | ENC p => 
-      let m' := pubkey_manifest_update p m in
-        aspid_manifest_update (enc_aspid) m'
+  | ENC p => aspid_manifest_update (enc_aspid) m
   | NULL => m 
   | CPY => m
   end.
-
-  (*
-Definition manifest_set_my_plc (p : Plc) (m : Manifest) : Manifest :=
-  let '{| my_abstract_plc := _ ;
-          asps := oldasps; 
-
-          uuidPlcs := oldKnowsOf; 
-          pubKeyPlcs := oldContext ; 
-          targetPlcs := oldTargets ;
-          policy := oldPolicy |} := m in
-  (Build_Manifest p oldasps old_app_asps oldKnowsOf oldContext oldTargets oldPolicy).
-  *)
 
 Definition manifest_update_env_res (p:Plc) (e:EnvironmentM) 
             (f:Manifest -> ResultT Manifest string) 
@@ -116,7 +40,7 @@ Definition manifest_update_env_res (p:Plc) (e:EnvironmentM)
   let m := 
     match (map_get e p) with
     | Some mm => mm
-    | None => (myPlc_manifest_update p empty_Manifest)
+    | None => empty_Manifest
     end 
   in
   match (f m) with
@@ -129,27 +53,15 @@ Definition manifest_update_env (p:Plc) (e:EnvironmentM)
   let m := 
     match (map_get e p) with
     | Some mm => mm
-    | None => (myPlc_manifest_update p empty_Manifest)
+    | None => empty_Manifest
     end in
-
-    let m' := (f m) in 
-      map_set e p m'.
-
-        
-Definition asp_manifest_generator (a:ASP) (p:Plc) (e:EnvironmentM) : EnvironmentM :=
-  manifest_update_env p e (asp_manifest_update a).
-
-Definition at_manifest_generator (fromPlc:Plc) (toPlc:Plc) 
-                                    (e:EnvironmentM) : EnvironmentM :=
-  manifest_update_env fromPlc e (knowsof_manifest_update toPlc).
-
+  let m' := (f m) in 
+    map_set e p m'.
 
 Fixpoint manifest_generator' (p:Plc) (t:Term) (e:EnvironmentM) : EnvironmentM :=
   match t with
-  | asp a => asp_manifest_generator a p e
-  | att q t' => 
-      let e' := at_manifest_generator p q e in 
-        manifest_generator' q t' e'
+  | asp a => manifest_update_env p e (asp_manifest_update a)
+  | att q t' => manifest_generator' q t' e
   | lseq t1 t2 => manifest_generator' p t2 (manifest_generator' p t1 e)
   | bseq _ t1 t2 => manifest_generator' p t2 (manifest_generator' p t1 e)
   | bpar _ t1 t2 => manifest_generator' p t2 (manifest_generator' p t1 e)
@@ -174,8 +86,7 @@ Lemma manifest_generator_never_empty : forall t p e,
   manifest_generator' p t e <> nil.
 Proof.
   induction t; simpl in *; intuition; eauto.
-  - destruct a; unfold asp_manifest_generator, 
-      manifest_update_env, asp_manifest_update in *; 
+  - destruct a; unfold manifest_update_env, asp_manifest_update in *; 
     repeat break_match; destruct e; simpl in *; try congruence;
     try (destruct p0; break_if; congruence);
     try (destruct p1; break_if; congruence).
@@ -187,49 +98,11 @@ Definition places_terms' (ts: list Term) (p:Plc) : list (list Plc) :=
 Definition places_terms (ts:list Term) (p:Plc) : list Plc :=
   dedup_list (List.concat (places_terms' ts p)).
 
-Definition fromSome{A:Type} (v:option A) (a:A) : A :=
-  match v with 
-  | Some v' => v'
-  | _ => a 
-  end.
-
-Definition get_manifest_env_default (e:EnvironmentM) (p:Plc) : Manifest :=
-  let m' := fromSome (map_get e p) empty_Manifest in
-    myPlc_manifest_update p m'.
-
-Definition get_unique_manifests_env' (ps:list Plc) (e:EnvironmentM) : list Manifest :=
-  List.map (get_manifest_env_default e) ps.
-
-Definition get_unique_manifests_env (ts: list Term) (p:Plc) (e:EnvironmentM) : list Manifest :=
-  let ps := places_terms ts p in
-    get_unique_manifests_env' ps e.
-
-Definition get_final_manifests_env (ts:list Term) (p:Plc) (e:EnvironmentM) : list Manifest :=
-  let ms := get_unique_manifests_env ts p e in 
-  let ms' := List.map (knowsof_myPlc_manifest_update) ms in
-  List.map (pubkeys_manifest_update (list_to_manset (places_terms ts p))) ms'.
-
-Definition man_gen_run (ts:list Term) (p:Plc) : EnvironmentM := manifest_generator_terms p ts.
-
 Definition environment_to_manifest_list (e:EnvironmentM) : list Manifest :=
   map_vals e.
 
-Definition demo_man_gen_run (ts:list Term) (p:Plc) : list Manifest := 
-  get_final_manifests_env ts p (man_gen_run ts p).
-
-Definition attify (t:Term) (p:Plc) : Term := 
-  att p t.
-
-Definition attify_terms' (pr:(Term * Plc)) : Term := 
-  match pr with 
-  | (t, p) => attify t p
-  end.
-
-Definition attify_terms (ls:list (Term * Plc)) : list Term :=
-  List.map attify_terms' ls.
-
-Fixpoint manifest_generator_app'' (et:Evidence) (al : AM_Library) (m:Manifest) 
-    : ResultT Manifest string :=
+Fixpoint manifest_generator_app'' (comp_map : ASP_Compat_MapT) 
+    (et:Evidence) (m:Manifest) : ResultT Manifest string :=
   match et with 
   | mt => resultC m 
   | nn _ => resultC m (* TODO: account for nonce handling here? *)
@@ -238,42 +111,42 @@ Fixpoint manifest_generator_app'' (et:Evidence) (al : AM_Library) (m:Manifest)
     | (EXTD n) => 
       match ps with 
       | asp_paramsC a _ targ _ =>
-        match (map_get (ASP_Compat_Map al) a) with
-        | Some a' => manifest_generator_app'' e' al (aspid_manifest_update a' m)
+        match (map_get comp_map a) with
+        | Some a' => 
+            manifest_generator_app'' comp_map e' (aspid_manifest_update a' m)
         | None => errC "Compatible Appraisal ASP not found in AM Library"%string
         end
       end 
     | ENCR => 
       match ps with 
       | asp_paramsC a _ p' _ =>
-        match (map_get (ASP_Compat_Map al) a) with
+        match (map_get comp_map a) with
         | Some a' => 
-            manifest_generator_app'' e' al (
-              aspid_manifest_update a' (pubkey_manifest_update p' m)
-            )
+            manifest_generator_app'' comp_map e' (aspid_manifest_update a' m)
         | None => errC "Compatible Appraisal ASP not found in AM Library"%string
         end
       end
     | KEEP => 
       let '(asp_paramsC a _ _ _) := ps in
-      match (map_get (ASP_Compat_Map al) a) with
+      match (map_get comp_map a) with
       | Some a' => 
-          manifest_generator_app'' e' al (aspid_manifest_update a' m)
+          manifest_generator_app'' comp_map e' (aspid_manifest_update a' m)
       | None => errC "Compatible Appraisal ASP not found in AM Library"%string
       end
     | _ => resultC m
     end
   | ss e1 e2 => 
-    match (manifest_generator_app'' e1 al m) with
-    | resultC m' => manifest_generator_app'' e2 al m'
+    match (manifest_generator_app'' comp_map e1 m) with
+    | resultC m' => manifest_generator_app'' comp_map e2 m'
     | errC e => errC e
     end
   end.
 
-Definition manifest_generator_app' (p:Plc) (et:Evidence) (al : AM_Library) (env:EnvironmentM) : ResultT EnvironmentM string :=
-  manifest_update_env_res p env (manifest_generator_app'' et al).
+Definition manifest_generator_app' (comp_map : ASP_Compat_MapT) (p:Plc) 
+    (et:Evidence) (env:EnvironmentM) : ResultT EnvironmentM string :=
+  manifest_update_env_res p env (manifest_generator_app'' comp_map et).
 
 
-Definition manifest_generator_app (et:Evidence) (p:Plc) (al : AM_Library)
-    : ResultT EnvironmentM string := 
-  manifest_generator_app' p et al e_empty.
+Definition manifest_generator_app (comp_map : ASP_Compat_MapT) 
+    (et:Evidence) (p:Plc) : ResultT EnvironmentM string := 
+  manifest_generator_app' comp_map p et e_empty.
