src/AM_Json_Interfaces.v
@@ -1,7 +1,7 @@
 Require Import List.
 Import ListNotations.
 Require Import BS Term_Defs Attestation_Session Interface String IO_Stubs Manifest_Admits ErrorStMonad_Coq AM_Monad Session_Config_Compiler Manifest.
-Require Import ErrorStringConstants AM_Helpers Impl_appraisal Cvm_Run.
+Require Import ErrorStringConstants AM_Helpers Impl_appraisal Cvm_Run AM_Manager.
 
 Definition am_check_auth_tok (t:Term) (fromPl:Plc) (authTok:ReqAuthTok) 
     : AM AppResultC :=
@@ -37,14 +37,14 @@ Definition am_serve_auth_tok_req (t:Term) (fromPl : Plc)
   | false => am_failm (am_error errStr_app_auth_tok)
   end. *)
 
-Definition do_appraisal_session (appreq:ProtocolAppraiseRequest) (m : Manifest) (aspBin : FS_Location) (nonceVal:BS)
+Definition do_appraisal_session (conf : AM_Manager_Config) (appreq:ProtocolAppraiseRequest) (nonceVal:BS)
     : ResultT ProtocolAppraiseResponse string :=
   let '(mkPAReq att_sess t p et ev) := appreq in
   let expected_et := eval t p et in 
   let app_am := gen_appraise_AM expected_et ev in 
   let init_noncemap := [(O, nonceVal)] in
   let init_nonceid := (S O) in
-  let sess_config := (session_config_compiler m aspBin att_sess) in
+  let sess_config := (session_config_compiler conf att_sess) in
   let my_amst := (mkAM_St init_noncemap init_nonceid sess_config) in
   match run_am_app_comp_init app_am my_amst with
   | errC e => errC e
@@ -52,8 +52,7 @@ Definition do_appraisal_session (appreq:ProtocolAppraiseRequest) (m : Manifest) 
       resultC (mkPAResp true appres)
   end.
 
-Definition handle_AM_request_JSON (js : JSON) (m : Manifest) (aspBin : FS_Location) (nonceVal:BS) 
-    : JSON :=
+Definition handle_AM_request_JSON (conf : AM_Manager_Config) (js : JSON) (nonceVal:BS) : JSON :=
   match (JSON_get_string STR_ACTION js) with
   | errC msg => ErrorResponseJSON msg
   | resultC req_type =>
@@ -63,7 +62,7 @@ Definition handle_AM_request_JSON (js : JSON) (m : Manifest) (aspBin : FS_Locati
       | errC msg => ErrorResponseJSON msg
       | resultC r =>
         let '(mkPRReq att_sess cop_term from_plc ev) := r in
-        let sc := (session_config_compiler m aspBin att_sess) in
+        let sc := (session_config_compiler conf att_sess) in
         let cvm_resp := (run_cvm_rawEv cop_term ev sc) in
         match cvm_resp with
         | errC e => ErrorResponseJSON e
@@ -81,7 +80,7 @@ Definition handle_AM_request_JSON (js : JSON) (m : Manifest) (aspBin : FS_Locati
       match (from_JSON js) with
       | errC msg => ErrorResponseJSON msg
       | resultC appreq =>
-        let app_resp := (do_appraisal_session appreq m aspBin nonceVal) in 
+        let app_resp := (do_appraisal_session conf appreq nonceVal) in 
         match app_resp with
         | errC e => ErrorResponseJSON e
         | resultC app_resp => to_JSON app_resp
