src/Manifest_JSON.v
@@ -1,100 +1,58 @@
 Require Import Stringifiable.
-Require Import JSON Manifest Manifest_Set Term_Defs_Core Manifest_JSON_Vars List ErrorStringConstants EqClass.
+Require Import JSON Manifest Manifest_Set Term_Defs_Core Manifest_JSON_Vars List ErrorStringConstants EqClass Maps.
 Import ListNotations ResultNotation.
 
 
 Definition Manifest_to_JSON (m : Manifest) : JSON :=
-  let '(Build_Manifest my_abstract_plc asps uuidPlcs pubKeyPlcs targetPlcs policy) := m 
+  let '(Build_Manifest asps asp_compat_map asp_fs_map policy) := m 
   in
     JSON_Object [
-      (MAN_ABS_PLC, 
-        (InJSON_String (to_string my_abstract_plc)));
       (MAN_ASPS, 
         (InJSON_Array (manifest_set_to_list_InJson asps)));
-      (MAN_UUID_PLCS, 
-        (InJSON_Array (manifest_set_to_list_InJson uuidPlcs)));
-      (MAN_PUBKEY_PLCS, 
-        (InJSON_Array (manifest_set_to_list_InJson pubKeyPlcs)));
-      (MAN_TARGET_PLCS, 
-        (InJSON_Array (manifest_set_to_list_InJson targetPlcs)));
+      (MAN_ASP_COMPAT_MAP, 
+        (InJSON_Object (to_JSON asp_compat_map)));
+      (MAN_ASP_FS_MAP, 
+        (InJSON_Object (to_JSON asp_fs_map)));
       (MAN_POLICY, 
         (InJSON_Array (manifest_set_pairs_to_list_InJson policy)))
     ].
 
 Definition JSON_to_Manifest (js : JSON) : ResultT Manifest string :=
-  temp_ABS_PLC <- JSON_get_string MAN_ABS_PLC js;;
   temp_ASPS <- JSON_get_Array MAN_ASPS js;;
-  temp_UUID_PLCS <- JSON_get_Array MAN_UUID_PLCS js;;
-  temp_PUBKEY_PLCS <- JSON_get_Array MAN_PUBKEY_PLCS js;;
-  temp_TARGET_PLCS <- JSON_get_Array MAN_TARGET_PLCS js;;
+  temp_ASP_COMPAT_MAP <- JSON_get_Object MAN_ASP_COMPAT_MAP js;;
+  temp_ASP_FS_MAP <- JSON_get_Object MAN_ASP_FS_MAP js;;
   temp_POLICY <- JSON_get_Array MAN_POLICY js;;
 
-  ABS_PLC <- from_string temp_ABS_PLC;;
   ASPS <- list_InJson_to_manifest_set temp_ASPS;;
-  UUID_PLCS <- list_InJson_to_manifest_set temp_UUID_PLCS;;
-  PUBKEY_PLCS <- list_InJson_to_manifest_set temp_PUBKEY_PLCS;;
-  TARGET_PLCS <- list_InJson_to_manifest_set temp_TARGET_PLCS;;
+  ASP_COMPAT_MAP <- from_JSON temp_ASP_COMPAT_MAP;;
+  ASP_FS_MAP <- from_JSON temp_ASP_FS_MAP;;
   POLICY <- list_InJson_to_manifest_set_pairs temp_POLICY;;
-  resultC (Build_Manifest ABS_PLC ASPS UUID_PLCS PUBKEY_PLCS TARGET_PLCS POLICY).
+  resultC (Build_Manifest ASPS ASP_COMPAT_MAP ASP_FS_MAP POLICY).
 
-Global Instance Jsonifiable_Manifest : Jsonifiable Manifest. 
+Global Instance Jsonifiable_Manifest `{Jsonifiable (MapC ASP_ID FS_Location), Jsonifiable (ASP_Compat_MapT)}: Jsonifiable Manifest. 
 eapply Build_Jsonifiable with 
-  (to_JSON := Manifest_to_JSON)
-  (from_JSON := JSON_to_Manifest).
-intuition; destruct a; simpl in *.
-unfold JSON_to_Manifest, res_bind; simpl in *;
-repeat (try break_match; simpl in *; subst; try find_injection; try find_rewrite; eauto; try congruence);
-repeat rewrite canonical_list_injson_to_manset in *;
-repeat rewrite canonical_list_injson_to_manset_pairs in *;
-try congruence; repeat find_injection; eauto.
-Defined.
+(to_JSON := (fun m =>
+  JSON_Object [
+    (MAN_ASPS, 
+      (InJSON_Array (manifest_set_to_list_InJson (asps m))));
+    (MAN_ASP_COMPAT_MAP, 
+      (InJSON_Object (to_JSON (ASP_Compat_Map m))));
+    (MAN_ASP_FS_MAP, 
+      (InJSON_Object (to_JSON (ASP_Mapping m))));
+    (MAN_POLICY, 
+      (InJSON_Array (manifest_set_pairs_to_list_InJson (man_policy m))))
+  ]))
+(from_JSON := (fun js =>
+    temp_ASPS <- JSON_get_Array MAN_ASPS js;;
+  temp_ASP_COMPAT_MAP <- JSON_get_Object MAN_ASP_COMPAT_MAP js;;
+  temp_ASP_FS_MAP <- JSON_get_Object MAN_ASP_FS_MAP js;;
+  temp_POLICY <- JSON_get_Array MAN_POLICY js;;
 
-Definition AM_Lib_to_JSON (am : AM_Library) : JSON :=
-  let '(Build_AM_Library clone_uuid lib_asps lib_plcs lib_pubkeys compat_asps_map) := am
-  in
-    JSON_Object [
-      (AM_CLONE_UUID, (InJSON_String (to_string clone_uuid)));
-      (AM_LIB_ASPS, (InJSON_Object (to_JSON lib_asps)));
-      (AM_LIB_PLCS, (InJSON_Object (to_JSON lib_plcs)));
-      (AM_LIB_PUBKEYS, (InJSON_Object (to_JSON lib_pubkeys)));
-      (AM_LIB_COMPAT_ASPS, (InJSON_Object (to_JSON compat_asps_map)))
-    ].
-
-Definition JSON_to_AM_Lib (js : JSON) : ResultT AM_Library string :=
-  temp_CLONE_UUID <- JSON_get_string AM_CLONE_UUID js;;
-  temp_LIB_ASPS <- JSON_get_Object AM_LIB_ASPS js;;
-  temp_LIB_PLCS <- JSON_get_Object AM_LIB_PLCS js;;
-  temp_LIB_PUBKEYS <- JSON_get_Object AM_LIB_PUBKEYS js;;
-  temp_COMPAT_ASPS <- JSON_get_Object AM_LIB_COMPAT_ASPS js;;
-
-  CLONE_UUID <- from_string temp_CLONE_UUID;;
-  LIB_ASPS <- from_JSON temp_LIB_ASPS;;
-  LIB_PLCS <- from_JSON temp_LIB_PLCS;;
-  LIB_PUBKEYS <- from_JSON temp_LIB_PUBKEYS;;
-  COMPAT_ASPS <- from_JSON temp_COMPAT_ASPS;;
-  resultC (Build_AM_Library CLONE_UUID LIB_ASPS LIB_PLCS LIB_PUBKEYS COMPAT_ASPS).
-
-Global Instance Jsonifiable_AM_Library : Jsonifiable AM_Library.
-eapply Build_Jsonifiable with
-  (to_JSON := AM_Lib_to_JSON)
-  (from_JSON := JSON_to_AM_Lib).
-intuition; destruct a; simpl in *.
-unfold JSON_to_AM_Lib, res_bind; simpl in *;
-repeat rewrite canonical_stringification in *;
-repeat (try break_match; simpl in *; subst; try find_injection; try find_rewrite; eauto; try congruence);
-try (repeat match goal with
-| H : result_map _ (map _ ?l) = errC _ |- _ => 
-    induction l; simpl in *; intuition; try congruence;
-    unfold res_bind in *; repeat (try break_match; simpl in *; subst; intuition; eauto; try find_injection; try find_rewrite; try congruence);
-    repeat rewrite canonical_stringification in *; congruence
-| H : result_map _ (map _ ?l) = resultC ?l' |- _ => 
-    let IH' := fresh "IH'" in
-    assert (l = l') by (
-      generalize dependent l';
-      induction l as [| ? l IH']; simpl in *; intuition; try congruence;
-      unfold res_bind in *; repeat (try break_match; simpl in *; subst; intuition; eauto; try find_injection; try find_rewrite; try congruence);
-      repeat rewrite canonical_stringification in *; try congruence;
-      repeat find_injection; eauto;
-      erewrite IH'; eauto); subst; clear H; eauto
-end; fail).
+  ASPS <- list_InJson_to_manifest_set temp_ASPS;;
+  ASP_COMPAT_MAP <- from_JSON temp_ASP_COMPAT_MAP;;
+  ASP_FS_MAP <- from_JSON temp_ASP_FS_MAP;;
+  POLICY <- list_InJson_to_manifest_set_pairs temp_POLICY;;
+  resultC (Build_Manifest ASPS ASP_COMPAT_MAP ASP_FS_MAP POLICY))).
+simpl_json; rewrite canonical_list_injson_to_manset;
+rewrite canonical_list_injson_to_manset_pairs; solve_json.
 Defined.
